there are some proofs in blocking programs

test-suite/iso/squiggle4Impl.v
@@ -38,12 +38,86 @@ Definition V := BinNums.positive.
 Definition Tm : Set := (@WTermSet V  Opid _).
 Definition BTm : Set := (V*Tm).
 
-Definition elimTerm (t:Tm) :  tmExt Tm BTm.
-  destruct t as [t p]. destruct t as [v | o lbt].
--  
-  match t with
-  |
-  |
-  
+Require Import Coq.btauto.Btauto.
+Require Import SquiggleEq.LibTactics.
 
-Definition Tm_R (t1 t2 : Tm)
+Definition elimTerm (t:Tm) :  tmExt Tm BTm.
+Proof.
+  destruct t as [t p].
+  destruct t as [v | o lbt]; [| destruct o]; simpl in p.
+  - exact evar.
+  - destruct lbt as [| b lbt]; try inverts p as p.
+    destruct b as [lv nt].
+    destruct lv as [| v lv]; try inverts p as p.
+    destruct lv as [|]; try inverts p as p.
+    destruct lbt as [|]; try inverts p as p.
+    cases (wft nt) as Ht;[| inverts p].
+    exact (@elam Tm BTm (v,(exist _ nt Ht))).
+  - destruct lbt as [| b lbt]; try inverts p as p.
+    destruct b as [lv f].
+    destruct lv as [|]; try inverts p as p.
+    destruct lbt as [| b lbt]; try inverts p as p.
+    destruct b as [lv a].
+    destruct lv as [|]; try inverts p as p.
+    destruct lbt as [|]; try inverts p as p.
+    cases (wft f) as Hf;[| inverts p].
+    cases (wft a) as Ha;[| inverts p].
+    exact (@eapp Tm BTm (exist _ f Hf) (exist _ a Ha)).
+  - destruct lbt as [|]; try inverts p as p.
+    exact (@enum Tm BTm n).
+Defined.    
+
+
+Definition applyBTerm (b:BTm) (u:Tm) :  Tm.
+Proof.
+  destruct b as (v,t).
+  exact (subst_wftset t v u).
+Defined.
+
+Require Import SquiggleEq.alphaeq.
+Definition Tm_R (t1 t2 :Tm) : Prop:= alpha_eq (proj1_sig t1) (proj1_sig t2).
+
+Definition BTm_R (bt1 bt2 :BTm) : Prop:=
+  let (v1, t1) := bt1 in
+  let (v2, t2) := bt2 in
+  alpha_eq_bterm (bterm [v1] (proj1_sig t1)) (bterm [v2] (proj1_sig t2)).
+
+
+Require Import squiggle4Thm.
+
+Check obsEqUni.
+      
+Lemma totalTm_R : TotalHeteroRel Tm_R.
+  split;  intros x; exists x; apply alpha_eq_refl.
+Defined.
+
+Lemma totalBTm_R : TotalHeteroRel BTm_R.
+  split;  intros x; exists x; destruct x; apply alphaeqbt_refl.
+Defined.
+
+Lemma elimTerm_R :
+   (forall (a1 : Tm) (a2 : Tm),
+        Tm_R a1 a2 ->
+        Top_squiggle4_tmExt_pmtcty_RR0 Tm Tm Tm_R BTm BTm BTm_R (elimTerm a1) (elimTerm a2)).
+Proof using.
+  intros ? ? Hr.
+  inverts Hr.
+  - destruct a1, a2. simpl in *. subst.
+    simpl. constructor.
+  - destruct a1, a2. simpl in *. subst.
+    rename w into p.
+    destruct op; simpl.
+    + destruct lbt1 as [| b lbt1]. try inverts p as p.
+      destruct b as [lv nt].
+      destruct lv as [| v lv]; try inverts p as p.
+      destruct lv as [|]; try inverts p as p.
+      destruct lbt1 as [|]; try inverts p as p.
+      simpl in *.
+      alphahypsd3.
+      simpl. unfold wf_term in p. simpl in p.
+      destruct p.
+      compute in p.
+  
+  simpl in Hr.
+  simpl.
+Check obsEqUni.
